From the dynamics of the resources (ex: $c_1$) at steady state:
$$\begin{align}
0 &= \delta (c^0_1 - c^*_1) - \frac{\mu_{11} c^*_1 }{Y_1} n^*_1 - \frac{\mu_{21} c^*_1 }{Y_1} n^*_2
\\
0 &= c^0_1 - c^*_1 - \frac{\mu_{11} c^*_1 }{Y_1 \delta} n^*_1 - \frac{\mu_{21} c^*_1}{Y_1 \delta} n^*_2
\\
0 &= \frac{c^0_1}{c^*_1} - 1 - \frac{\mu_{11}}{Y_1 \delta} n^*_1 - \frac{\mu_{21}}{Y_1 \delta} n^*_2
\\
\frac{\mu_{11}}{Y_1 \delta} n^*_1 + \frac{\mu_{21}}{Y_1 \delta} n^*_2 &= \frac{c^0_1}{c^*_1} - 1
\\
\mu_{11} n^*_1 + \mu_{21} n^*_2 &= \Big(\frac{c^0_1}{c^*_1} - 1 \Big) Y_1 \delta
\end{align}$$

